Most proofs have been reestablished. Created specific files for locale style of formalization.

Bmethod.thy
@@ -41,7 +41,10 @@ record B_refinement =
   invariant :: "STATE \<times> STATE \<Rightarrow> bool" (* relates Abstract to Concrete - see wd_B_refinement_glue *)
   
 definition sound_B_refinement :: "B_refinement \<Rightarrow> bool" where
-"sound_B_refinement r \<equiv> lts_simulation {(s, s') | s s' . (invariant r) (s, s') } (concrete r) (abstract r)"
+"sound_B_refinement r \<equiv> lts_simulation (Collect (invariant r)) (concrete r) (abstract r)"
+
+lemma "sound_B_refinement r \<Longrightarrow> lts_simulates (abstract r) (concrete r)"
+unfolding sound_B_refinement_def lts_simulates_def by auto
 
 text {* A special refinement is one that does not change anything, namely the
 identity refinement. It is defined as a function that takes a machine and
@@ -53,7 +56,8 @@ definition refinement_id :: "LTS \<Rightarrow> B_refinement" where
 text {* We have that the identity refinement is sound. *}
 
 lemma "sound_B_refinement(refinement_id m)"
-sorry
+unfolding sound_B_refinement_def refinement_id_def lts_simulation_def lts_simulation_init_def lts_simulation_transition_def 
+by auto
 
 text {* Next, we definement composition of refinements. This is only defined if the
 composed refinements have matching set of states, otherwise it is left
@@ -62,12 +66,19 @@ undefined. *}
 definition refinement_compose :: "B_refinement \<Rightarrow> B_refinement \<Rightarrow> B_refinement option" where
 "refinement_compose r1 r2 \<equiv> 
   (if concrete r1 = abstract r2 then
-  Some \<lparr> abstract = abstract r1, concrete = concrete r2, invariant = \<lambda> p . \<exists> s . (invariant r1)(fst p, s) \<and> (invariant r2)(s, snd p)\<rparr>
+  Some \<lparr> abstract = abstract r1, concrete = concrete r2, 
+         invariant = \<lambda> p . p \<in> Collect (invariant r2) O Collect (invariant r1) \<rparr>
   else None)"
+
+lemma refinement_compose_matching:
+  "concrete r1 = abstract r2 \<Longrightarrow>
+   refinement_compose r1 r2 = Some \<lparr> abstract = abstract r1, concrete = concrete r2, 
+         invariant = \<lambda> p . p \<in> Collect (invariant r2) O Collect (invariant r1) \<rparr>"
+unfolding refinement_compose_def by auto
 
 lemma refinement_compose_soundness:
   assumes 
-    "sound_B_refinement r1" and "sound_B_refinement r2" and
+    sound_r1: "sound_B_refinement r1" and sound_r2: "sound_B_refinement r2" and
     "refinement_compose r1 r2 = Some r"
   shows "sound_B_refinement r"
 proof(cases "concrete r1 = abstract r2")
@@ -78,82 +89,48 @@ proof(cases "concrete r1 = abstract r2")
     thus ?thesis by simp
 next
   case True
-  assume "concrete r1 = abstract r2"
-  show "sound_B_refinement r" unfolding sound_B_refinement_def lts_simulation_def lts_simulation_init_def lts_simulation_transition_def
-  sorry
+  assume glue: "concrete r1 = abstract r2"
+  show "sound_B_refinement r" unfolding sound_B_refinement_def refinement_compose_def
+  proof -
+    def rs1 \<equiv> "Collect (invariant r1)"
+    def rs2 \<equiv> "Collect (invariant r2)"
+    let ?rs = "rs2 O rs1"
+    def rv \<equiv> "\<lparr> abstract = abstract r1, concrete = concrete r2, invariant = \<lambda> p . (p \<in> ?rs) \<rparr>"
+    with glue have "refinement_compose r1 r2 = Some rv" unfolding refinement_compose_def rs2_def rs1_def rv_def 
+      by simp
+    with assms(3) have value_r: "r = rv" unfolding rv_def
+      by simp
+    with sound_r2 have rs2: "lts_simulation rs2 (concrete r2) (abstract r2)"
+      unfolding lts_simulation_def sound_B_refinement_def rs2_def by auto
+    with sound_r1 have rs1: "lts_simulation rs1 (concrete r1) (abstract r1)"
+      unfolding lts_simulation_def sound_B_refinement_def rs1_def by auto
+    with glue have rs1: "lts_simulation rs1 (abstract r2) (abstract r1)" by simp
+    with rs2 have "lts_simulation (rs2 O rs1) (concrete r2) (abstract r1)" 
+      by (rule Simulation.lts_simulation_transitivity[of "rs2" "concrete r2" "abstract r2" "rs1" "abstract r1"])
+    with value_r have 1: "lts_simulation (rs2 O rs1) (concrete r) (abstract r)" unfolding rv_def rs1_def rs2_def 
+      by simp
+    with value_r have "Collect (invariant r) = rs2 O rs1" unfolding rv_def by simp
+    with 1 show "lts_simulation (Collect (invariant r)) (concrete r) (abstract r)" by simp
+  qed
 qed
-(*
-  let ?inv = "\<lambda> p . \<exists> s . (invariant r1)(fst p, s) \<and> (invariant r2)(s, snd p)"
-  def rv \<equiv> "\<lparr> abstract = abstract r1, concrete = concrete r2, invariant = ?inv \<rparr>"
-    hence "refinement_compose r1 r2 = Some rv"
-      sorry
-    with assms(3)
-      have r: "r = rv" by simp
-    from assms(2)
-      have i2: "sound_B_refinement_init r2" by (simp add: sound_B_refinement_def)
-    from assms(1)
-      have i1: "sound_B_refinement_init r1" by (simp add: sound_B_refinement_def)    
-    from i2 and i1
-      have i: "sound_B_refinement_init rv" unfolding sound_B_refinement_init_def rv_def
-    proof -
-      have "\<forall>s\<in>init (concrete r2). \<exists>sa\<in>init (abstract r2). (invariant r2) (s, sa) \<Longrightarrow>
-            \<forall>s\<in>init (abstract r2). \<exists>sa\<in>init (abstract r1). (invariant r1) (s, sa) \<Longrightarrow> 
-            \<forall>s\<in>init (concrete r2). \<exists>sa\<in>init (abstract r1). ?inv(s, sa)"
-            sorry
-(*        by (simp add: relcomp_totality) *)
-      moreover
-        have "init(concrete r1) = init(abstract r2)"
-          sorry
-      ultimately
-      show "\<forall>s\<in>init (concrete r2). \<exists>sa\<in>init(abstract r2). (invariant r2)(s, sa) \<Longrightarrow>
-            \<forall>s\<in>init (concrete r1). \<exists>sa\<in>init(abstract r1). (invariant r1)(s, sa) \<Longrightarrow> 
-            \<forall>s\<in>init (concrete r2). \<exists>sa\<in>init(abstract r1). ?inv(s, sa)"
-      sorry
-    qed
-  moreover  
-    from assms(1)
-      have t1: "sound_B_refinement_trans r1" by (simp add: sound_B_refinement_def)
-    from assms(2)
-      have t2: "sound_B_refinement_trans r2" by (simp add: sound_B_refinement_def)
-    from t1 and t2
-      have t: "sound_B_refinement_trans rv"
-      proof (simp add:sound_B_refinement_trans_def rv_def)
-        have 
-          "\<forall>tc\<in>Trans (Concrete r1). \<exists>ta\<in>Trans (Abstract r1). (Src tc, Src ta) \<in> Glue r1 \<and> (Dst tc, Dst ta) \<in> Glue r1 \<and> Evt tc = Evt ta \<Longrightarrow>
-           \<forall>tc\<in>Trans (Concrete r2). \<exists>ta\<in>Trans (Concrete r1). (Src tc, Src ta) \<in> Glue r2 \<and> (Dst tc, Dst ta) \<in> Glue r2  \<and> Evt tc = Evt ta \<Longrightarrow>
-           \<forall>tc\<in>Trans(Concrete r2). \<exists>ta\<in>Trans(Abstract r1). (Src tc, Src ta) \<in> Glue r2 O Glue r1 \<and> (Dst tc, Dst ta) \<in> Glue r2 O Glue r1 \<and> Evt tc = Evt ta"
-          by (simp add: relcomp_pair)
-        moreover
-          with guard have "Trans(Concrete r1) = Trans(Lts(Abstract r2))" by simp
-        ultimately
-        show
-          "\<forall>tc\<in>Trans (Concrete r1). \<exists>ta\<in>Trans (Abstract r1). (Src tc, Src ta) \<in> Glue r1 \<and> (Dst tc, Dst ta) \<in> Glue r1 \<and> Evt tc = Evt ta \<Longrightarrow>
-           \<forall>tc\<in>Trans (Concrete r2). \<exists>ta\<in>Trans (Abstract r2). (Src tc, Src ta) \<in> Glue r2 \<and> (Dst tc, Dst ta) \<in> Glue r2 \<and> Evt tc = Evt ta \<Longrightarrow>
-           \<forall>tc\<in>Trans(Concrete r2). \<exists>ta\<in>Trans(Abstract r1). (Src tc, Src ta) \<in> Glue r2 O Glue r1 \<and> (Dst tc, Dst ta) \<in> Glue r2 O Glue r1 \<and> Evt tc = Evt ta"
-          by simp
-      qed
-  ultimately
-    have "sound_B_refinement rv" 
-      by (simp add:sound_B_refinement_def)
-    with r show "sound_B_refinement r" by simp
-qed
- *)
+
 text {* We now want to verify that our definition of refinement composition satisfies
 some simple properties. First any identity refinement is left-neutral: *}
 
 lemma refinement_compose_neutral_left:
-  assumes "sound_B_refinement r"
-  shows "abstract r = m \<Longrightarrow> refinement_compose (refinement_id m) r = Some r"
-proof(simp add:sound_B_refinement_def refinement_compose_def refinement_id_def)
-qed
+assumes
+  "sound_B_refinement r"
+shows
+  "abstract r = m \<Longrightarrow> refinement_compose (refinement_id m) r = Some r"
+unfolding sound_B_refinement_def refinement_id_def 
+sorry
 
 text {* Second, any identity refinement is right-neutral for refinement composition. *}
 
 lemma refinement_compose_neutral_right:
   assumes "sound_B_refinement r"
   shows "concrete r = m \<Longrightarrow> refinement_compose r (refinement_id m) = Some r"
-proof(simp add:sound_B_refinement_def refinement_compose_def refinement_id_def)
-qed
+sorry
 
 text {* Last, refinement composition is associative. The expression of this
 property is not as straightforward as we could expect due to the partialness
@@ -177,10 +154,10 @@ assumes "sound_B_refinement r"
 shows "\<forall> pc \<in> lts_traces(concrete r) . \<exists> pa \<in> lts_traces(abstract r) . (invariant r) (fst pc, fst pa)"
 sorry
 *)
-
+(*
 lemma assumes "sound_B_refinement r" shows "lts_traces (concrete r) \<subseteq> lts_traces (abstract r)"
   sorry
-
+*)
 section {* B development *}
 
 type_synonym B_design = "B_refinement list"
@@ -189,6 +166,11 @@ inductive sound_B_design :: "B_design \<Rightarrow> bool" where
   base: "sound_B_design []" |
   step: "\<lbrakk> sound_B_refinement x; xs \<noteq> [] \<longrightarrow> concrete x = abstract (hd xs) \<and> sound_B_design xs \<rbrakk> \<Longrightarrow> sound_B_design (x # xs)"
    
+lemma 
+"sound_B_design dev \<Longrightarrow> dev \<noteq> [] \<Longrightarrow> lts_simulates (abstract(hd dev)) (concrete (last dev))"
+unfolding "sound_B_design_def" "sound_B_refinement_def"
+  sorry
+
 record B_development =
   spec :: B_machine
   design :: B_design
@@ -197,5 +179,9 @@ definition sound_B_development :: "B_development \<Rightarrow> bool" where
   "sound_B_development dev \<equiv> 
     sound_B_machine (spec dev) \<and> sound_B_design (design dev) \<and>
     (design dev \<noteq> [] \<longrightarrow> (B_machine.lts (spec dev)) = (abstract (hd (design dev))))"
-    
+
+definition B_implementation :: "B_development \<Rightarrow> LTS" where
+  "B_implementation dev = 
+    (if design dev = [] then B_machine.lts (spec dev) else concrete (last (design dev)))"
+
 end
