Simulation.thy
@@ -15,9 +15,9 @@ definition lts_simulation_init :: "STATE rel \<Rightarrow> LTS \<Rightarrow> LTS
 
 definition lts_simulation_transition :: "STATE rel \<Rightarrow> LTS \<Rightarrow> LTS \<Rightarrow> bool" where
   "lts_simulation_transition r l1 l2 \<equiv> 
-    \<forall> s1 \<in> states l1 . \<forall> s2 \<in> states l2 . (s1, s2) \<in> r \<longrightarrow>
+    \<forall> s1 s2 . (s1, s2) \<in> r \<longrightarrow>
       (\<forall> t1 \<in> trans l1 . src t1 = s1 \<longrightarrow>
-        (\<exists> t2 \<in> trans l2 . (src t2 = s2 \<and> evt t1 = evt t2 \<and> (dst t1, dst t2) \<in> r)))"
+        (\<exists> t2 \<in> trans l2 . src t2 = s2 \<and> evt t1 = evt t2 \<and> (dst t1, dst t2) \<in> r))"
 
 definition lts_simulation :: "STATE rel \<Rightarrow> LTS \<Rightarrow> LTS \<Rightarrow> bool" where
   "lts_simulation r l1 l2 \<equiv> lts_simulation_init r l1 l2 \<and> lts_simulation_transition r l1 l2"
@@ -36,9 +36,60 @@ qed
 text {* Second, we have that the composition of two simulation relations 
 is a simulation relation. *}
 lemma lts_simulation_transitivity:
-  "lts_simulation r12 l1 l2 \<and> lts_simulation r23 l2 l3 \<Longrightarrow> lts_simulation (r23 O r12) l1 l3"
-  unfolding lts_simulation_def lts_simulation_init_def lts_simulation_transition_def relcomp_def 
-sorry
+assumes s12: "lts_simulation r12 l1 l2" and s23: "lts_simulation r23 l2 l3"
+shows "lts_simulation (r12 O r23) l1 l3"
+proof -
+  have "lts_simulation_init (r12 O r23) l1 l3"
+  proof -
+    from s12 have "lts_simulation_init r12 l1 l2" unfolding lts_simulation_def ..
+  moreover
+    from s23 have "lts_simulation_init r23 l2 l3" unfolding lts_simulation_def ..
+  ultimately
+    show "lts_simulation_init (r12 O r23) l1 l3" unfolding lts_simulation_init_def relcomp_def by blast
+  qed
+moreover
+  have "lts_simulation_transition (r12 O r23) l1 l3" unfolding "lts_simulation_transition_def"
+  proof
+    fix s1
+    show "\<forall>s3. (s1, s3) \<in> r12 O r23 \<longrightarrow> (\<forall>t1\<in>LTS.trans l1. src t1 = s1 \<longrightarrow> (\<exists>t2\<in>LTS.trans l3. src t2 = s3 \<and> evt t1 = evt t2 \<and> (dst t1, dst t2) \<in> r12 O r23))"
+    proof
+      fix s3
+      show "(s1, s3) \<in> r12 O r23 \<longrightarrow> (\<forall>t1\<in>LTS.trans l1. src t1 = s1 \<longrightarrow> (\<exists>t2\<in>LTS.trans l3. src t2 = s3 \<and> evt t1 = evt t2 \<and> (dst t1, dst t2) \<in> r12 O r23))"
+      proof
+        assume 1: "(s1, s3) \<in> r12 O r23"
+        show "(\<forall>t1\<in>LTS.trans l1. src t1 = s1 \<longrightarrow> (\<exists>t2\<in>LTS.trans l3. src t2 = s3 \<and> evt t1 = evt t2 \<and> (dst t1, dst t2) \<in> r12 O r23))"
+        proof
+          fix t1
+          assume dom_t1: "t1\<in>LTS.trans l1"
+          show "src t1 = s1 \<longrightarrow> (\<exists>t3\<in>LTS.trans l3. src t3 = s3 \<and> evt t1 = evt t3 \<and> (dst t1, dst t3) \<in> r12 O r23)"
+          proof
+            assume src_t1: "src t1 = s1"
+            show "\<exists>t3\<in>LTS.trans l3. src t3 = s3 \<and> evt t1 = evt t3 \<and> (dst t1, dst t3) \<in> r12 O r23"
+              proof-
+                have "\<exists> t3 . t3 \<in> LTS.trans l3 \<and> src t3 = s3 \<and> evt t1 = evt t3 \<and> (dst t1, dst t3) \<in> r12 O r23"
+                proof -
+                  from 1 have "\<exists> s2 . (s1, s2) \<in> r12 \<and> (s2, s3) \<in> r23" unfolding relcomp_def by auto
+                  then obtain s2 where 2: "(s1, s2) \<in> r12 \<and> (s2, s3) \<in> r23" ..
+                moreover
+                  from 2 have "(s1, s2) \<in> r12" ..
+                  with s12 src_t1 dom_t1 obtain t2 where w12: "t2 \<in> LTS.trans l2 \<and> src t2 = s2 \<and> evt t1 = evt t2 \<and> (dst t1, dst t2) \<in> r12" 
+                    unfolding lts_simulation_def lts_simulation_transition_def by blast
+                moreover
+                  from 2 have "(s2, s3) \<in> r23" by simp
+                  with s23 w12 obtain w where "w \<in> LTS.trans l3 \<and> src w = s3 \<and> evt t2 = evt w \<and> (dst t2, dst w) \<in> r23" 
+                    unfolding lts_simulation_def lts_simulation_transition_def by blast
+                  with w12 have "w \<in> LTS.trans l3 \<and> src w = s3 \<and> evt t1 = evt w \<and> (dst t1, dst w) \<in> r12 O r23" unfolding relcomp_def by auto
+                  then show ?thesis ..
+                qed
+              then show ?thesis by auto
+            qed
+          qed
+        qed
+      qed
+    qed
+  qed
+  ultimately show ?thesis unfolding lts_simulation_def ..
+qed
 
 text {* Next we carry these properties over to the simulates relation over LTS. *}
 
@@ -57,20 +108,15 @@ assumes
   s12: "l1 \<sim> l2" and s23: "l2 \<sim> l3"
 shows
   "l1 \<sim> l3"
-unfolding lts_simulates_def
-sorry
-
-(*
-proof
-  from s12 obtain r where "lts_simulation r l2 l1" unfolding lts_simulates_def ..
-moreover
+proof -
   from s23 obtain s where "lts_simulation s l3 l2" unfolding lts_simulates_def ..
+moreover
+  from s12 obtain r where "lts_simulation r l2 l1" unfolding lts_simulates_def ..
 ultimately
-  obtain x where "x = r O s"
-    sorry
-  from this show "lts_simulation x l3 l1"
-    sorry
+  have "lts_simulation (s O r) l3 l1" 
+    by (rule lts_simulation_transitivity[of "s" "l3" "l2" "r" "l1"])
+  then have "\<exists> r . lts_simulation r l3 l1" ..
+  then show ?thesis unfolding lts_simulates_def by simp
 qed
-*)
   
 end
