LocaleLTS.thy
@@ -1,0 +1,91 @@
+theory LocaleLTS
+
+imports Main
+
+begin
+
+section {* Labelled transition systems *}
+
+text {* The semantics of a B component is a discrete, eventful, state-transition systems. We 
+first define what is meant exactly by such systems. Any system is, at a given time in a state. 
+Conversely, a system has a set of possible states. A system evolves from state to state,
+and such changes called transitions. Also when a system makes a transition, this is observable
+and this observation is called an event. State, transition and event are three different
+entities and a type is declared for each: *}
+
+locale Transition =
+fixes 
+  src :: "'trans \<Rightarrow> 'state" and
+  dst :: "'trans \<Rightarrow> 'state" and
+  evt :: "'trans \<Rightarrow> 'event"
+  
+locale LTS = Transition src dst evt 
+for
+  src :: "'trans \<Rightarrow> 'state" and
+  dst :: "'trans \<Rightarrow> 'state" and
+  evt :: "'trans \<Rightarrow> 'event"
++
+fixes
+  init :: "'state set" and
+  trans :: "'trans set"
+begin
+
+  inductive_set states :: "'state set" where
+      base[elim!]: "s \<in> init \<Longrightarrow> s \<in> states"
+    | step[elim!]: "\<lbrakk> t \<in> trans; src t \<in> states \<rbrakk> \<Longrightarrow> dst t \<in> states"
+
+  definition successors :: "'state set \<Rightarrow> 'state set" where
+    "successors S \<equiv> { s | s . \<exists> t \<in> trans . src t \<in> S \<and> dst t = s}"
+  
+  lemma reachable_init: "init \<subseteq> states" by auto
+
+  lemma reachable_stable: "successors states \<subseteq> states"
+    unfolding successors_def by auto
+
+text {* The following lemma is related to the identification of sufficient conditions to establish 
+safety properties. Consider a property that is satisfied by some set of states $S$. If the initial 
+states are in $S$, and if the successors of $S$ are in $S$ then all the reachable states are in 
+$S$. *}
+
+  lemma reachable_induct_set:
+    assumes base: "init \<subseteq> S" and step: "successors S \<subseteq> S"
+    shows "states \<subseteq> S"
+  proof
+    fix x
+    assume "x \<in> states"
+    thus "x \<in> S"
+    proof (induct x)
+      fix i
+      assume "i \<in> init"
+      with base show "i \<in> S" ..
+    next
+      fix t
+      assume "t \<in> trans" "src t \<in> states" "src t \<in> S"
+      with step show "dst t \<in> S" unfolding successors_def by auto
+    qed
+  qed
+
+text {* Next we enunciate and prove a similar lemma for predicates. *}
+
+lemma reachable_induct_predicate:
+  assumes base: "\<forall> s \<in> init . p s" and 
+          step: "\<forall> t \<in> trans . p (src t) \<longrightarrow> p (dst t)"
+  shows "\<forall> s \<in> states . p s"
+proof
+  fix x
+  assume "x \<in> states" 
+  thus "p x"
+  proof (induct x)
+    fix i
+    assume "i \<in> init"
+    with base show "p i" ..
+  next
+    fix t
+    assume "t \<in> trans" "src t \<in> states" "p (src t)"
+    with step show "p (dst t)" unfolding successors_def by auto
+  qed
+qed
+
+end
+
+end
